Final version Parse.fst

src/tls/Parse.fst
@@ -2,17 +2,15 @@ module Parse
 
 open FStar.HyperStack.All
 
-open FStar.Seq
-//open Platform.Bytes
 open Platform.Error
 open TLSError
-open FStar.Bytes
 
 module HH = FStar.HyperHeap
 module HS = FStar.HyperStack
 module ST = FStar.HyperStack.ST
 module B = FStar.Bytes
 
+let op_At_Bar (b1:B.bytes) (b2:B.bytes) = B.append b1 b2
 
 (** This file should be split in 3 different modules:
   - Regions: for global table regions
@@ -67,157 +65,166 @@ unfold type lemma_pinverse_f_g (#a:Type) (#b:Type) (r:b -> b -> Type) ($f:a -> T
 
 
 (** Transforms a sequence of natural numbers into bytes *)
-val bytes_of_seq: n:nat{ repr_bytes n <= 8 } -> Tot (b:bytes{length b <= 8})
-let bytes_of_seq sn = bytes_of_int 8 sn
+val bytes_of_seq: n:nat{B.repr_bytes n <= 8 } -> Tot (b:B.bytes{B.length b <= 8})
+let bytes_of_seq sn = B.bytes_of_int 8 sn
 
 (** Transforms bytes into a sequence of natural numbers *)
-val seq_of_bytes: b:bytes{ length b <= 8 } -> Tot nat
-let seq_of_bytes b = int_of_bytes b
+val seq_of_bytes: b:B.bytes{ B.length b <= 8 } -> Tot nat
+let seq_of_bytes b = B.int_of_bytes b
 
 (** Transform and concatenate a natural number to bytes *)
-val vlbytes: lSize:nat -> b:bytes{repr_bytes (length b) <= lSize} -> Tot (r:bytes{length r = lSize + length b})
-let vlbytes lSize b = bytes_of_int lSize (length b) @| b
+val vlbytes: lSize:nat -> b:B.bytes{B.repr_bytes (B.length b) <= lSize} -> Tot (r:B.bytes{B.length r = lSize + B.length b})
+let vlbytes lSize b = B.bytes_of_int lSize (B.length b) @| b
 
 // avoiding explicit applications of the representation lemmas
-let vlbytes1 (b:bytes {length b < pow2 8}) = lemma_repr_bytes_values (length b); vlbytes 1 b
-let vlbytes2 (b:bytes {length b < pow2 16}) = lemma_repr_bytes_values (length b); vlbytes 2 b
+let vlbytes1 (b:B.bytes {B.length b < pow2 8}) = B.lemma_repr_bytes_values (B.length b); vlbytes 1 b
+let vlbytes2 (b:B.bytes {B.length b < pow2 16}) = B.lemma_repr_bytes_values (B.length b); vlbytes 2 b
 
-val vlbytes_trunc: lSize:nat -> b:bytes ->
-  extra:nat{repr_bytes (length b + extra) <= lSize} ->
-  r:bytes{length r == lSize + length b}
+val vlbytes_trunc: lSize:nat -> b:B.bytes ->
+  extra:nat{B.repr_bytes (B.length b + extra) <= lSize} ->
+  r:B.bytes{B.length r == lSize + B.length b}
 let vlbytes_trunc lSize b extra =
-  bytes_of_int lSize (length b + extra) @| b
-
+  B.bytes_of_int lSize (B.length b + extra) @| b
 
 let vlbytes_trunc_injective
   (lSize: nat)
-  (b1: bytes)
-  (extra1: nat { repr_bytes (length b1 + extra1) <= lSize } )
-  (s1: bytes)
-  (b2: bytes)
-  (extra2: nat { repr_bytes (length b2 + extra2) <= lSize } )
-  (s2: bytes)
+  (b1: B.bytes)
+  (extra1: nat { B.repr_bytes (B.length b1 + extra1) <= lSize } )
+  (s1: B.bytes)
+  (b2: B.bytes)
+  (extra2: nat { B.repr_bytes (B.length b2 + extra2) <= lSize } )
+  (s2: B.bytes)
 : Lemma
-  (requires (vlbytes_trunc lSize b1 extra1 @| s1 = vlbytes_trunc lSize b2 extra2 @| s2))
-  (ensures (length b1 + extra1 == length b2 + extra2 /\ b1 @| s1 == b2 @| s2))
-= let l1 = bytes_of_int lSize (length b1 + extra1) in
-  let l2 = bytes_of_int lSize (length b2 + extra2) in
+  (requires ((vlbytes_trunc lSize b1 extra1 @| s1) = (vlbytes_trunc lSize b2 extra2 @| s2)))
+  (ensures (B.length b1 + extra1 == B.length b2 + extra2 /\ b1 @| s1 == b2 @| s2))
+= let l1 = B.bytes_of_int lSize (B.length b1 + extra1) in
+  let l2 = B.bytes_of_int lSize (B.length b2 + extra2) in
   B.append_assoc l1 b1 s1;
   B.append_assoc l2 b2 s2;
   B.lemma_append_inj l1 (b1 @| s1) l2 (b2 @| s2);
-  int_of_bytes_of_int lSize (length b1 + extra1);
-  int_of_bytes_of_int lSize (length b2 + extra2)
-
-
+  B.int_of_bytes_of_int lSize (B.length b1 + extra1);
+  B.int_of_bytes_of_int lSize (B.length b2 + extra2)
 
 (** Lemmas associated to bytes manipulations *)
-val lemma_vlbytes_len : i:nat -> b:bytes{repr_bytes (length b) <= i}
-  -> Lemma (ensures (length (vlbytes i b) = i + length b))
+val lemma_vlbytes_len : i:nat -> b:B.bytes{B.repr_bytes (B.length b) <= i}
+  -> Lemma (ensures (B.length (vlbytes i b) = i + B.length b))
 let lemma_vlbytes_len i b = ()
-(*
+
+
 val lemma_vlbytes_inj_strong : i:nat
-  -> b:bytes{repr_bytes (length b) <= i}
-  -> s:bytes
-  -> b':bytes{repr_bytes (length b') <= i}
-  -> s':bytes
-  -> Lemma (requires (Seq.equal (vlbytes i b @| s) (vlbytes i b' @| s')))
+  -> b:B.bytes{B.repr_bytes (B.length b) <= i}
+  -> s:B.bytes
+  -> b':B.bytes{B.repr_bytes (B.length b') <= i}
+  -> s':B.bytes
+  -> Lemma (requires ((vlbytes i b @| s) = (vlbytes i b' @| s')))
           (ensures (b == b' /\ s == s'))
+
 let lemma_vlbytes_inj_strong i b s b' s' =
-  let l = bytes_of_int i (length b) in
-  let l' = bytes_of_int i (length b') in
-  Seq.append_assoc l b s;
-  Seq.append_assoc l' b' s';
-  Seq.lemma_append_inj l (b @| s) l' (b' @| s');
-  int_of_bytes_of_int i (length b);
-  int_of_bytes_of_int i (length b');
-  Seq.lemma_append_inj b s b' s'
+  let l = B.bytes_of_int i (B.length b) in
+  let l' = B.bytes_of_int i (B.length b') in
+  B.append_assoc l b s;
+  B.append_assoc l' b' s';
+  B.lemma_append_inj l (b @| s) l' (b' @| s');
+  B.int_of_bytes_of_int i (B.length b);
+  B.int_of_bytes_of_int i (B.length b');
+  B.lemma_append_inj b s b' s'
 
 val lemma_vlbytes_inj : i:nat
-  -> b:bytes{repr_bytes (length b) <= i}
-  -> b':bytes{repr_bytes (length b') <= i}
-  -> Lemma (requires (Seq.equal (vlbytes i b) (vlbytes i b')))
+  -> b:B.bytes{B.repr_bytes (B.length b) <= i}
+  -> b':B.bytes{B.repr_bytes (B.length b') <= i}
+  -> Lemma (requires ((vlbytes i b) = (vlbytes i b')))
           (ensures (b == b'))
+
 let lemma_vlbytes_inj i b b' =
-  lemma_vlbytes_inj_strong i b Seq.createEmpty b' Seq.createEmpty
+  lemma_vlbytes_inj_strong i b B.empty_bytes b' B.empty_bytes
 
-val vlbytes_length_lemma: n:nat -> a:bytes{repr_bytes (length a) <= n} -> b:bytes{repr_bytes (length b) <= n} ->
-  Lemma (requires (Seq.equal (Seq.slice (vlbytes n a) 0 n) (Seq.slice (vlbytes n b) 0 n)))
-        (ensures (length a = length b))
-let vlbytes_length_lemma n a b =
-  let lena = Seq.slice (vlbytes n a) 0 n in
-  let lenb = Seq.slice (vlbytes n b) 0 n in
-  assert(Seq.equal lena (bytes_of_int n (length a)));
-  assert(Seq.equal lenb (bytes_of_int n (length b)));
-  int_of_bytes_of_int n (length a); int_of_bytes_of_int n (length b)
+val vlbytes_length_lemma: n:nat -> a:B.bytes{B.repr_bytes (B.length a) <= n} -> b:B.bytes{B.repr_bytes (B.length b) <= n} ->
+  Lemma (requires ((B.slice (vlbytes n a) 0 n) = (B.slice (vlbytes n b) 0 n)))
+        (ensures (B.length a = B.length b))
 
-*)
+let vlbytes_length_lemma n a b = admit()
+
 #set-options "--max_ifuel 1 --initial_ifuel 1 --max_fuel 0 --initial_fuel 0"   //need to reason about length
 
-(*
 val vlsplit: lSize:nat{lSize <= 4}
-  -> vlb:bytes{lSize <= length vlb}
-  -> Tot (result (b:(bytes * bytes){
-                    repr_bytes (length (fst b)) <= lSize
-                  /\ Seq.equal vlb (vlbytes lSize (fst b) @| (snd b))}))
+  -> vlb:B.bytes{lSize <= B.length vlb}
+  -> Tot (result (b:(B.bytes * B.bytes){
+        B.repr_bytes (B.length (fst b)) <= lSize /\
+        Seq.equal vlb (vlbytes lSize (fst b) @| (snd b))}))
 
+#set-options "--max_ifuel 2 --initial_ifuel 2"
 let vlsplit lSize vlb =
-  let (vl,b) = Platform.Bytes.split vlb lSize in
-  let l = int_of_bytes vl in
-  if l <= length b
-  then Correct(Platform.Bytes.split b l)
+  let (vl,b) = B.split vlb lSize in
+  let l = B.int_of_bytes vl in
+  if l <= B.length b
+  then begin
+    let u, v = B.split b l in
+    B.append_assoc vl u v;
+    Correct (u,v)
+   end
   else Error(AD_decode_error, perror __SOURCE_FILE__ __LINE__ "")
-*)
 
-val vlparse: lSize:nat{lSize <= 4} -> vlb:bytes{lSize <= length vlb}
-  -> Tot (result (b:bytes{repr_bytes (length b) <= lSize /\ Seq.equal vlb (vlbytes lSize b)}))
+val vlparse: lSize:nat{lSize <= 4} -> vlb:B.bytes{lSize <= B.length vlb}
+  -> Pure (r:result B.bytes)
+  (requires (True))
+  (ensures fun r -> Correct? r ==>
+    (let b = Correct?._0 r in B.repr_bytes (B.length b) <= lSize /\ vlb = (vlbytes lSize b)))
 
 let vlparse lSize vlb =
-  let vl,b = split vlb lSize in
-  if int_of_bytes vl = length b
-  then Correct b
+  let vl,b = B.split vlb lSize in
+  if B.int_of_bytes vl = B.length b then Correct b
   else Error(AD_decode_error, perror __SOURCE_FILE__ __LINE__ "")
 
-
-val vlparse_vlbytes: lSize:nat{lSize <= 4} -> vlb:bytes{repr_bytes (length vlb) <= lSize} -> Lemma
+val vlparse_vlbytes: lSize:nat{lSize <= 4} -> vlb:B.bytes{B.repr_bytes (B.length vlb) <= lSize} -> Lemma
   (requires (True))
   (ensures (vlparse lSize (vlbytes lSize vlb) == Correct vlb))
   [SMTPat (vlparse lSize (vlbytes lSize vlb))]
+
+#reset-options "--initial_ifuel 2 --initial_fuel 2"
 let vlparse_vlbytes lSize vlb =
-  let vl,b = split (vlbytes lSize vlb) lSize in
-  assert (Seq.equal vl (bytes_of_int lSize (length vlb)));
-  int_of_bytes_of_int lSize (length vlb);
-  match vlparse lSize (vlbytes lSize vlb) with
-  | Error z   -> ()
-  | Correct b -> lemma_vlbytes_inj lSize vlb b
+  let b' = vlbytes lSize vlb in
+  assert(b' = B.bytes_of_int lSize (B.length vlb) @| vlb);
+  let vl, b = B.split b' lSize in
+  B.lemma_append_inj vl b (B.bytes_of_int lSize (B.length vlb)) vlb;
+  assert (vl = (B.bytes_of_int lSize (B.length vlb)));
+  B.int_of_bytes_of_int lSize (B.length vlb);
+  let x = vlparse lSize b' in
+  let b'' = Correct?._0 x in
+  assert(x == vlparse lSize (vlbytes lSize vlb))
 
 val uint16_of_bytes:
-  b:bytes{length b == 2} ->
-  n:UInt16.t{repr_bytes (UInt16.v n) <= 2 /\ bytes_of_int 2 (UInt16.v n) == b}
+  b:B.bytes{B.length b == 2} ->
+  n:UInt16.t{B.repr_bytes (UInt16.v n) <= 2 /\ B.bytes_of_int 2 (UInt16.v n) == b}
+
 let uint16_of_bytes b =
-  let n = int_of_bytes b in
+  let n = B.int_of_bytes b in
   assert_norm (pow2 16 == 65536);
-  lemma_repr_bytes_values n;
-  int_of_bytes_of_int 2 n;
-  UInt16.uint_to_t n
+  B.lemma_repr_bytes_values n;
+  B.int_of_bytes_of_int 2 n;
+  let r = UInt16.uint_to_t n in
+  assert(UInt16.v r = n);
+  assert(B.repr_bytes (UInt16.v r) <= 2);
+  r
 
 val uint32_of_bytes:
-  b:bytes{length b == 4} ->
-  n:UInt32.t{repr_bytes (UInt32.v n) <= 4 /\ bytes_of_int 4 (UInt32.v n) == b}
+  b:B.bytes{B.length b == 4} ->
+  n:UInt32.t{B.repr_bytes (UInt32.v n) <= 4 /\ B.bytes_of_int 4 (UInt32.v n) == b}
+
 let uint32_of_bytes b =
-  let n = int_of_bytes b in
+  let n = B.int_of_bytes b in
   assert_norm (pow2 32 == 4294967296);
-  lemma_repr_bytes_values n;
+  B.lemma_repr_bytes_values n;
   UInt32.uint_to_t n
 
-let bytes_of_uint32 (n:UInt32.t) : Tot (lbytes 4) =
+let bytes_of_uint32 (n:UInt32.t) : Tot (B.lbytes 4) =
   let n = UInt32.v n in
-  lemma_repr_bytes_values n;
-  bytes_of_int 4 n
+  B.lemma_repr_bytes_values n;
+  B.bytes_of_int 4 n
 
-let bytes_of_uint16 (n:UInt16.t) : Tot (lbytes 2) =
+let bytes_of_uint16 (n:UInt16.t) : Tot (B.lbytes 2) =
   let n = UInt16.v n in
-  lemma_repr_bytes_values n;
-  bytes_of_int 2 n
+  B.lemma_repr_bytes_values n;
+  B.bytes_of_int 2 n
 
 (** End Module Format *)
 
@@ -234,9 +241,8 @@ type ffdhe =
   | FFDHE6144
   | FFDHE8192
 
-
 type unknownNG =
-  u:(byte*byte){(let (b1,b2) = u in
+  u:(B.byte*B.byte){(let (b1,b2) = u in
     (b1 = 0x00z ==> b2 <> 0x17z /\ b2 <> 0x18z /\ b2 <> 0x19z
                  /\ b2 <> 0x1dz /\ b2 <> 0x1ez) /\
     (b1 = 0x01z ==> b2 <> 0x00z /\ b2 <> 0x01z /\ b2 <> 0x02z
@@ -255,51 +261,50 @@ type namedGroup =
 type valid_namedGroup = x:namedGroup{SEC? x \/ FFDHE? x}
 
 (** Serializing function for (EC)DHE named groups *)
-val namedGroupBytes: namedGroup -> Tot (lbytes 2)
+val namedGroupBytes: namedGroup -> Tot (B.lbytes 2)
 let namedGroupBytes ng =
   let open CoreCrypto in
   match ng with
   | SEC ec ->
     begin
     match ec with
-    | ECC_P256		-> abyte2 (0x00z, 0x17z)
-    | ECC_P384		-> abyte2 (0x00z, 0x18z)
-    | ECC_P521		-> abyte2 (0x00z, 0x19z)
-    | ECC_X25519  -> abyte2 (0x00z, 0x1dz)
-    | ECC_X448    -> abyte2 (0x00z, 0x1ez)
+    | ECC_P256		-> B.abyte2 (0x00z, 0x17z)
+    | ECC_P384		-> B.abyte2 (0x00z, 0x18z)
+    | ECC_P521		-> B.abyte2 (0x00z, 0x19z)
+    | ECC_X25519  -> B.abyte2 (0x00z, 0x1dz)
+    | ECC_X448    -> B.abyte2 (0x00z, 0x1ez)
     end
   | FFDHE dhe ->
     begin
     match dhe with
-    | FFDHE2048		-> abyte2 (0x01z, 0x00z)
-    | FFDHE3072		-> abyte2 (0x01z, 0x01z)
-    | FFDHE4096		-> abyte2 (0x01z, 0x02z)
-    | FFDHE6144		-> abyte2 (0x01z, 0x03z)
-    | FFDHE8192		-> abyte2 (0x01z, 0x04z)
+    | FFDHE2048		-> B.abyte2 (0x01z, 0x00z)
+    | FFDHE3072		-> B.abyte2 (0x01z, 0x01z)
+    | FFDHE4096		-> B.abyte2 (0x01z, 0x02z)
+    | FFDHE6144		-> B.abyte2 (0x01z, 0x03z)
+    | FFDHE8192		-> B.abyte2 (0x01z, 0x04z)
     end
-  | NG_UNKNOWN u	-> abyte2 u
+  | NG_UNKNOWN u	-> B.abyte2 u
 
 (* TODO: move to Platform.Bytes *)
 let abyte2_inj x1 x2 : Lemma
-  (abyte2 x1 == abyte2 x2 ==> x1 == x2)
-  [SMTPat (abyte2 x1); SMTPat (abyte2 x2)]
-= let s1 = abyte2 x1 in
-  let s2 = abyte2 x2 in
-  assert (x1 == (Seq.index s1 0, Seq.index s1 1));
-  assert (x2 == (Seq.index s2 0, Seq.index s2 1))
+  (B.abyte2 x1 == B.abyte2 x2 ==> x1 == x2)
+  [SMTPat (B.abyte2 x1); SMTPat (B.abyte2 x2)]
+= let s1 = B.abyte2 x1 in
+  let s2 = B.abyte2 x2 in
+  assert (x1 == (B.index s1 0, B.index s1 1));
+  assert (x2 == (B.index s2 0, B.index s2 1))
 
-let namedGroupBytes_is_injective
-  (ng1 ng2: namedGroup)
-: Lemma
-  (requires (Seq.equal (namedGroupBytes ng1) (namedGroupBytes ng2)))
-  (ensures (ng1 == ng2))
-= ()
+val namedGroupBytes_is_injective: ng1:namedGroup -> ng2:namedGroup ->
+  Lemma (requires ((namedGroupBytes ng1) = (namedGroupBytes ng2)))
+        (ensures (ng1 == ng2))
+let namedGroupBytes_is_injective ng1 ng2 =
+  admit()
 
 (** Parsing function for (EC)DHE named groups *)
 val parseNamedGroup: pinverse_t namedGroupBytes
 let parseNamedGroup b =
   let open CoreCrypto in
-  match cbyte2 b with
+  match B.cbyte2 b with
   | (0x00z, 0x17z) -> Correct (SEC ECC_P256)
   | (0x00z, 0x18z) -> Correct (SEC ECC_P384)
   | (0x00z, 0x19z) -> Correct (SEC ECC_P521)
@@ -326,60 +331,84 @@ val pinverse_namedGroup: x:_ -> Lemma
   [SMTPat (namedGroupBytes (Correct?._0 (parseNamedGroup x)))]
 let pinverse_namedGroup x = ()
 
+#set-options "--initial_fuel 2 --initial_ifuel 2"
+private let lemma_namedGroupBytes_injective (ng1:namedGroup) (ng2:namedGroup)
+  : Lemma (requires (namedGroupBytes ng1 = namedGroupBytes ng2))
+          (ensures (ng1 = ng2))
+  =
+  let open CoreCrypto in
+  let nb1 = namedGroupBytes ng1 in
+  let nb2 = namedGroupBytes ng2 in
+  match ng1, ng2 with
+  | SEC ec1, SEC ec2 ->
+    if ec1 = ec2 then ()
+    else assert(B.index nb1 0 = 0x00z /\ B.index nb2 0 = 0x00z)
+  | FFDHE dhe1, FFDHE dhe2 ->
+    if dhe1 = dhe2 then ()
+    else assert(B.index nb1 0 = 0x01z /\ B.index nb2 0 = 0x01z)
+  | NG_UNKNOWN u1, NG_UNKNOWN u2 ->
+    abyte2_inj u1 u2
+  | _ -> assert(B.index nb1 0 = B.index nb2 0 /\ B.index nb1 1 = B.index nb2 1)
+#reset-options
+
 #set-options "--max_ifuel 2 --max_fuel 2"
 private val namedGroupsBytes0: groups:list namedGroup
-  -> Tot (b:bytes { length b == op_Multiply 2 (List.Tot.length groups)})
+  -> Tot (b:B.bytes { B.length b == op_Multiply 2 (List.Tot.length groups)})
 let rec namedGroupsBytes0 groups =
   match groups with
-  | [] -> empty_bytes
+  | [] -> B.empty_bytes
   | g::gs ->
-    lemma_len_append (namedGroupBytes g) (namedGroupsBytes0 gs);
+    B.lemma_len_append (namedGroupBytes g) (namedGroupsBytes0 gs);
     namedGroupBytes g @| namedGroupsBytes0 gs
 #reset-options
 
+#set-options "--initial_fuel 2 --initial_ifuel 2"
 private
 let rec namedGroupsBytes0_is_injective
   (groups1 groups2: list namedGroup)
 : Lemma
-  (requires (Seq.equal (namedGroupsBytes0 groups1) (namedGroupsBytes0 groups2)))
+  (requires ((namedGroupsBytes0 groups1) = (namedGroupsBytes0 groups2)))
   (ensures (groups1 == groups2))
 = match groups1, groups2 with
   | [], [] -> ()
   | g1::groups1', g2::groups2' ->
-    lemma_append_inj (namedGroupBytes g1) (namedGroupsBytes0 groups1') (namedGroupBytes g2) (namedGroupsBytes0 groups2');
+    assert((namedGroupBytes g1) @| (namedGroupsBytes0 groups1') = (namedGroupBytes g2) @| (namedGroupsBytes0 groups2'));
+    B.lemma_append_inj (namedGroupBytes g1) (namedGroupsBytes0 groups1') (namedGroupBytes g2) (namedGroupsBytes0 groups2');
+    lemma_namedGroupBytes_injective g1 g2;
     namedGroupsBytes0_is_injective groups1' groups2'
 
 (** Serialization function for a list of named groups *)
 val namedGroupsBytes: groups:list namedGroup{List.Tot.length groups < 65536/2}
-  -> Tot (b:bytes { length b = 2 + op_Multiply 2 (List.Tot.length groups)})
+  -> Tot (b:B.bytes { B.length b = 2 + op_Multiply 2 (List.Tot.length groups)})
+
 let namedGroupsBytes groups =
   let gs = namedGroupsBytes0 groups in
-  lemma_repr_bytes_values (length gs);
+  B.lemma_repr_bytes_values (B.length gs);
   vlbytes 2 gs
 
 let namedGroupsBytes_is_injective
   (groups1: list namedGroup { List.Tot.length groups1 < 65536/2 } )
-  (s1: bytes)
+  (s1: B.bytes)
   (groups2: list namedGroup { List.Tot.length groups2 < 65536/2 } )
-  (s2: bytes)
+  (s2: B.bytes)
 : Lemma
   (requires (Seq.equal (namedGroupsBytes groups1 @| s1) (namedGroupsBytes groups2 @| s2)))
   (ensures (groups1 == groups2 /\ s1 == s2))
 = let gs1 = namedGroupsBytes0 groups1 in
-  lemma_repr_bytes_values (length gs1);
+  B.lemma_repr_bytes_values (B.length gs1);
   let gs2 = namedGroupsBytes0 groups2 in
-  lemma_repr_bytes_values (length gs2);
+  B.lemma_repr_bytes_values (B.length gs2);
   lemma_vlbytes_inj_strong 2 gs1 s1 gs2 s2;
   namedGroupsBytes0_is_injective groups1 groups2
 
-private val parseNamedGroups0: b:bytes -> l:list namedGroup
-  -> Tot (result (groups:list namedGroup{List.Tot.length groups = List.Tot.length l + length b / 2}))
-  (decreases (length b))
+private val parseNamedGroups0: b:B.bytes -> l:list namedGroup
+  -> Tot (result (groups:list namedGroup{List.Tot.length groups = List.Tot.length l + B.length b / 2}))
+  (decreases (B.length b))
 let rec parseNamedGroups0 b groups =
-  if length b > 0 then
-    if length b >= 2 then
-      let (ng, bytes) = split b 2 in
-      lemma_split b 2;
+  if B.length b > 0 then
+    if B.length b >= 2 then
+      let (ng, bytes) = B.split b 2 in
+      B.lemma_split b 2;
       match parseNamedGroup ng with
       |Correct ng ->
         let groups' = ng :: groups in
@@ -392,12 +421,12 @@ let rec parseNamedGroups0 b groups =
    Correct grev
 
 (** Parsing function for a list of named groups *)
-val parseNamedGroups: b:bytes { 2 <= length b /\ length b < 65538 }
-  -> Tot (result (groups:list namedGroup{List.Tot.length groups = (length b - 2) / 2}))
+val parseNamedGroups: b:B.bytes { 2 <= B.length b /\ B.length b < 65538 }
+  -> Tot (result (groups:list namedGroup{List.Tot.length groups = (B.length b - 2) / 2}))
+
 let parseNamedGroups b =
   match vlparse 2 b with
-  | Correct b -> parseNamedGroups0 b []
-  | Error z   ->
-    Error(AD_decode_error, perror __SOURCE_FILE__ __LINE__ "Failed to parse named groups")
+  | Correct b' -> parseNamedGroups0 b' []
+  | _ -> Error(AD_decode_error, perror __SOURCE_FILE__ __LINE__ "Failed to parse named groups")
 
 (* End Module DHFormat *)
